pass on style

src/equations.v
@@ -16,7 +16,7 @@ From RDF Require Export Rdf Triple Term Util IsoCan.
 
 Section Template.
   Variable disp : unit.
-(* TODO : check that order is needed, since below comes a comparison comp on graphs *)
+  (* TODO : check that order is needed, since below comes a comparison comp on graphs *)
   Variable I B L : orderType disp.
   Notation le_triple := (@le_triple disp I B L).
 
@@ -25,33 +25,33 @@ Section Template.
   Hypothesis nat_inj : nat -> B.
   Hypothesis nat_inj_ : injective nat_inj.
 
-  (* comparison on graphs, morally an order relation. 
+  (* comparison on graphs, morally an order relation.
      TODO : we can relax all assumptions on cmp/choose_graph to the relabelling of
-    the graph to be canonized, is it relevant? *)
-    Variable (cmp : seq (triple I B L) -> seq (triple I B L) -> bool).
-    
-    Definition choose_graph (g1 g2 : seq (triple I B L)) :=
-      if cmp g1 g2 then g2 else g1.
+     the graph to be canonized, is it relevant? *)
+  Variable (cmp : seq (triple I B L) -> seq (triple I B L) -> bool).
 
-    Hypothesis choose_graphA : associative choose_graph.
-    Hypothesis choose_graphC : commutative choose_graph.
-    Hypothesis choose_graph_idem : idempotent choose_graph.
+  Definition choose_graph (g1 g2 : seq (triple I B L)) :=
+    if cmp g1 g2 then g2 else g1.
 
-    (* A default graph *)
-   Variable can : seq (triple I B L).
-   Hypothesis ucan : uniq can.
-   Hypothesis sort_can : sort le_triple can = can.
+  Hypothesis choose_graphA : associative choose_graph.
+  Hypothesis choose_graphC : commutative choose_graph.
+  Hypothesis choose_graph_idem : idempotent choose_graph.
+
+  (* A default graph *)
+  Variable can : seq (triple I B L).
+  Hypothesis ucan : uniq can.
+  Hypothesis sort_can : sort le_triple can = can.
   (* Determines a choice of default graph can *)
-   Hypothesis gbot_lid : left_id can choose_graph.
+  Hypothesis gbot_lid : left_id can choose_graph.
 
-   HB.instance Definition _ :=
-   Monoid.isComLaw.Build
-     (seq (triple I B L)) can
-     (choose_graph) choose_graphA
-     choose_graphC
-     gbot_lid.
+  HB.instance Definition _ :=
+    Monoid.isComLaw.Build
+      (seq (triple I B L)) can
+      (choose_graph) choose_graphA
+      choose_graphC
+      gbot_lid.
 
-(* Hash maps as sequences of pairs of a b-node and a hash *)
+  (* Hash maps as sequences of pairs of a b-node and a hash *)
   Definition hash_map := seq (B * nat).
   (* Initial hash map from a graph *)
   Definition bnodes_hm (hm : hash_map): seq B := map fst hm.
@@ -59,88 +59,92 @@ Section Template.
   Variable (init_hash : seq (triple I B L) -> hash_map).
   (* init_hash g has the same bnodes as the graph g *)
   Hypothesis good_init :
-  forall (g : seq (triple I B L)), bnodes_hm (init_hash g) =i get_bts g.
+    forall (g : seq (triple I B L)), bnodes_hm (init_hash g) =i get_bts g.
 
-(* Type of an element of a partition *)
+  (* Type of an element of a partition *)
   Definition part := seq (B * nat).
-(* Pick a part p from a failed attempt at computing a fine partition from the input hashmap hm. Expected:
-- (map fst p) is included in (map fst hm) 
-- elements of p have the same hash 
-- p is non empty and non singleton *)
-Variable choose_part : hash_map -> part.
-(* all nodes in choose_part hm lead to bnodes of hm, but with possibly changed hashes.
-   remember the list of bnodes of a graph is unique *)
- Hypothesis in_part_in_bnodes : forall bn hm, bn \in choose_part hm -> bn.1 \in bnodes_hm hm.
+  (* Pick a part p from a failed attempt at computing a fine partition from the input hashmap hm. Expected:
+     - (map fst p) is included in (map fst hm)
+     - elements of p have the same hash
+     - p is non empty and non singleton *)
+  Variable choose_part : hash_map -> part.
+  (* all nodes in choose_part hm lead to bnodes of hm, but with possibly changed hashes.
+     remember the list of bnodes of a graph is unique *)
+  Hypothesis in_part_in_bnodes :
+    forall bn hm, bn \in choose_part hm -> bn.1 \in bnodes_hm hm.
 
- 
-(* Type of partitions *)
+
+  (* Type of partitions *)
   Definition partition := seq part.
-(* TODO : remove *)
+  (* TODO : remove *)
   Definition pred_eq {T : eqType} (t: T):= fun t'=> t == t'.
-(* Tests whether the hash of p is n *)
+  (* Tests whether the hash of p is n *)
   Definition eq_hash (n : nat) (p: B * nat) := pred_eq n p.2.
-(* Tests whether the node of p is b *) 
+  (* Tests whether the node of p is b *)
   Definition eq_bnode (b : B) (p: B * nat) := pred_eq b p.1.
-(* splits hm according to hash n *)
+  (* splits hm according to hash n *)
   Definition partitionate (n : nat) (hm : hash_map) :=
     (filter (eq_hash n) hm, filter (negb \o eq_hash n) hm).
 
-(* update a hashmap from an input graph, without increasing the measure *)
-Variables (color color_refine : seq (triple I B L) -> hash_map -> hash_map).
+  (* update a hashmap from an input graph, without increasing the measure *)
+  Variables (color color_refine : seq (triple I B L) -> hash_map -> hash_map).
 
-(* coloring a hashmap of a graph using the same graph does not change its bnodes 
-  TODO : Pick one of the versions, color_bnodes is stronger but may be not needed.
-*)
-Hypothesis color_good_hm :
+  (* coloring a hashmap of a graph using the same graph does not change its bnodes
+     TODO : Pick one of the versions, color_bnodes is stronger but may be not needed. *)
+  Hypothesis color_good_hm :
     forall (g : seq (triple I B L)) hm,
       bnodes_hm hm =i get_bts g -> bnodes_hm (color g hm) =i get_bts g.
-(* Hypothesis color_bnodes : forall (g : seq (triple I B L)) hm, bnodes_hm (color g hm) =i bnodes_hm hm. *)
+  (* Hypothesis color_bnodes : forall (g : seq (triple I B L)) hm, bnodes_hm (color g hm) =i bnodes_hm hm. *)
 
-(* Same for color_refine *)
-Hypothesis color_refine_good_hm :
+  (* Same for color_refine *)
+  Hypothesis color_refine_good_hm :
     forall (g : seq (triple I B L)) hm,
-               bnodes_hm hm =i get_bts g -> bnodes_hm (color_refine g hm) =i get_bts g.
+      bnodes_hm hm =i get_bts g -> bnodes_hm (color_refine g hm) =i get_bts g.
 
- (* Marks a bnode in a hashmap*)
-Variable (mark : B -> hash_map -> hash_map).
-(* Marking a hashmap with one of its bnodes does not change its bnodes (but only the hashes)*)
-Hypothesis good_mark : forall (g : seq (triple I B L)) (hm : hash_map), 
-       bnodes_hm hm =i get_bts g -> forall b, b \in bnodes_hm hm -> bnodes_hm (mark b hm) =i get_bts g.
-(* TODO : to be simplified into 
-    Hypothesis good_mark : forall (hm : hash_map), 
+  (* Marks a bnode in a hashmap*)
+  Variable (mark : B -> hash_map -> hash_map).
+  (* Marking a hashmap with one of its bnodes does not change its bnodes (but only the hashes)*)
+  Hypothesis good_mark :
+    forall (g : seq (triple I B L)) (hm : hash_map),
+      bnodes_hm hm =i get_bts g ->
+      forall b, b \in bnodes_hm hm -> bnodes_hm (mark b hm) =i get_bts g.
+  (* TODO : to be simplified into
+    Hypothesis good_mark : forall (hm : hash_map),
      forall b, b \in bnodes_hm hm -> bnodes_hm (mark b hm) =i bnodes_hm hm.
-*)
- 
-(* Measure on hash_map*)
-Variable (M : hash_map -> nat).
+   *)
 
-(* Mark decreases the measure *)
-Hypothesis (markP : forall (bn : B * nat) (hm : hash_map), bn \in choose_part hm -> M (mark bn.1 hm) < M hm).
-(* color_refine does not increase the measure *)
-Hypothesis (color_refineP : forall (g : seq (triple I B L)) (hm : hash_map) , M (color_refine g hm) <= M hm).
+  (* Measure on hash_map*)
+  Variable (M : hash_map -> nat).
 
-(* TODO: remove this local def *)
-Local Definition n0 := 0.
+  (* Mark decreases the measure *)
+  Hypothesis markP :
+    forall (bn : B * nat) (hm : hash_map),
+      bn \in choose_part hm -> M (mark bn.1 hm) < M hm.
+  (* color_refine does not increase the measure *)
+  Hypothesis color_refineP :
+    forall (g : seq (triple I B L)) (hm : hash_map) ,
+      M (color_refine g hm) <= M hm.
 
-Definition fun_of_hash_map (hm : hash_map) : B -> B :=
+  (* TODO: remove this local def *)
+  Definition fun_of_hash_map (hm : hash_map) : B -> B :=
     fun b =>
       if has (eq_bnode b) hm then
-        let the_label := nth n0 (map snd hm) (find (eq_bnode b) hm) in
+        let the_label := nth O (map snd hm) (find (eq_bnode b) hm) in
         nat_inj the_label
       else
         b.
 
-Hypothesis iso_color_fine_can : forall (g h : seq (triple I B L)),
-uniq g -> uniq h ->
-effective_iso_ts g h ->
-relabeling_seq_triple (fun_of_hash_map (color g (init_hash g))) g
-=i relabeling_seq_triple (fun_of_hash_map (color h (init_hash h))) h.
+  Hypothesis iso_color_fine_can :
+    forall (g h : seq (triple I B L)),
+      uniq g -> uniq h ->
+      effective_iso_ts g h ->
+         relabeling_seq_triple (fun_of_hash_map (color g (init_hash g))) g
+      =i relabeling_seq_triple (fun_of_hash_map (color h (init_hash h))) h.
 
-
-  Lemma size_filter {T : Type} (f : T -> bool) (l : seq T) : size (filter f l ) <= size l.
-  Proof. elim: l=> // hd tl IHl /=. case (f hd)=> //.
-         have /(_ (size tl)) H : forall n, n < n.+1 by apply ltnSn.
-         by apply (Order.POrderTheory.le_le_trans IHl H).
+  Lemma size_filter_le {T : Type} (f : T -> bool) (l : seq T) : size (filter f l ) <= size l.
+  Proof.
+  elim: l=> // hd tl IHl /=.
+  by case: ifP=> [//| _]; apply (leq_trans IHl).
   Qed.
 
   Lemma nat_coq_nat (n m : nat) :  (n < m)%nat = (n < m). Proof. by []. Qed.
@@ -148,51 +152,48 @@ relabeling_seq_triple (fun_of_hash_map (color g (init_hash g))) g
 
   Equations? gen_partition (hm : hash_map) : partition by wf (size hm) lt :=
     gen_partition nil := nil;
-    gen_partition (bn::l) := ((partitionate bn.2 (bn::l)).1) :: gen_partition (partitionate bn.2 (bn::l)).2 .
+    gen_partition (bn::l) :=
+      ((partitionate bn.2 (bn::l)).1) :: gen_partition (partitionate bn.2 (bn::l)).2.
   Proof.
     rewrite /= /eq_hash/pred_eq/negb /= eqxx /=.
-    have H := size_filter ((fun b : bool => if b then false else true) \o (fun p : B * nat => n == p.2)) l.
-    apply /ltP.
-    by apply : leq_trans H _.
+    have H := size_filter_le ((fun b : bool => if b then false else true) \o (fun p : B * nat => n == p.2)) l.
+    by apply /ltP; apply : leq_trans H _.
   Qed.
 
   Definition is_trivial (p : part) : bool := size p == 1.
   Definition is_fine (P : partition) : bool := all is_trivial P.
-  
-  
   Definition hashes_hm (hm : hash_map): seq nat :=
     map snd hm.
 
-    Equations? foldl_In {T R : eqType} (s : seq T) (f : R -> forall (y : T), y \in s -> R) (z : R) : R :=
+  Equations? foldl_In {T R : eqType} (s : seq T) (f : R -> forall (y : T), y \in s -> R) (z : R) : R :=
     foldl_In nil f z := z;
     foldl_In (a :: l) f z := foldl_In l (fun x y inP=> f x y _) (f z a _).
   Proof.
-    by rewrite in_cons inP orbT.
-    by rewrite in_cons eqxx.
+  by rewrite in_cons inP orbT.
+  by rewrite in_cons eqxx.
   Qed.
 
   Lemma foldl_foldl_eq {T R : eqType} (s : list T) (f : R -> T -> R) z :
-    @foldl_In _ _ s (fun r t (_ : t \in s) => f r t) z = foldl f z s.
+    @foldl_In _ _ s (fun (r:R) (t:T) (_ : t \in s) => f r t) z = foldl f z s.
   Proof.
-    funelim (foldl_In s _ z).
-    - by [].
-    - autorewrite with foldl_In; apply H.
+  funelim (foldl_In s _ z).
+  - by [].
+  - autorewrite with foldl_In; apply H.
   Qed.
 
   Section Distinguish.
 
-    
     Lemma bnodes_hm_exists (hm : hash_map) :
       forall b, b \in bnodes_hm hm -> exists n, (b,n) \in hm.
     Proof.
-      move=> b /mapP/=[[b' n] bin ->]/=. by exists n.
+    by move=> b /mapP/=[[b' n] bin ->]/=; exists n.
     Qed.
 
     Lemma bnodes_hm_has_eq_bnodes (hm : hash_map) :
-        forall b, b \in bnodes_hm hm -> has (eq_bnode b) hm.
+      forall b, b \in bnodes_hm hm -> has (eq_bnode b) hm.
     Proof.
     move=> b /bnodes_hm_exists/=[n bnin].
-    apply /hasP. exists (b,n)=> //.
+    apply /hasP; exists (b,n)=> //.
     by rewrite /eq_bnode/pred_eq eqxx.
     Qed.
 
@@ -200,22 +201,22 @@ relabeling_seq_triple (fun_of_hash_map (color g (init_hash g))) g
       size s = size bs ->
       find (eq_bnode bn) (zip bs s) = index bn bs.
     Proof.
-      elim: bs s => [| a l IHl]; first by move=> ?; rewrite zip0s.
-      by case =>  [//| b l2] /= [eqsize_tl]; rewrite eq_sym IHl //.
+    elim: bs s => [| a l IHl]; first by move=> ?; rewrite zip0s.
+    by case =>  [//| b l2] /= [eqsize_tl]; rewrite eq_sym IHl //.
     Qed.
 
     Lemma find_index_eq_hash bs s (bn : nat) :
       size s = size bs ->
       find (eq_hash bn) (zip bs s) = index bn s.
     Proof.
-      elim: s bs => [| a l IHl]; first by move=> ?; rewrite zips0.
-      by case => [//| b l2] /= [eqsize_tl]; rewrite eq_sym IHl //.
+    elim: s bs => [| a l IHl] bs; first by move=> ?; rewrite zips0.
+    by case: bs => [//| b l2] /= [eqsize_tl]; rewrite eq_sym IHl //.
     Qed.
 
     Lemma rem_swap (T : eqType) (s : seq T) (x y : T):
       rem x (rem y s) = rem y (rem x s).
     Proof.
-    elim: s=> [//| h tl IHtl]. rewrite /=.
+    elim: s=> [//| h tl IHtl] /=.
     case: ifP.
     + move=> /eqP eqhy; rewrite eqhy.
       case: ifP; first by move /eqP ->.
@@ -225,13 +226,15 @@ relabeling_seq_triple (fun_of_hash_map (color g (init_hash g))) g
     Qed.
 
     Lemma hm_zip (hm : hash_map): hm = zip (map fst hm) (map snd hm).
-    Proof. rewrite zip_map; elim: hm => [//| [h1 h2] tl IHtl] /=; by rewrite -IHtl. Qed.
+    Proof. by rewrite zip_map; elim: hm => [//| [h1 h2] tl IHtl] /=; rewrite -IHtl. Qed.
 
-    Lemma size_proj (T1 T2 : Type) (s : seq (T1 * T2)) : size [seq i.2 | i <- s] = size [seq i.1 | i <- s].
+    Lemma size_proj (T1 T2 : Type) (s : seq (T1 * T2)) :
+      size [seq i.2 | i <- s] = size [seq i.1 | i <- s].
     Proof. by elim: s=> [//| h tl IHtl] /=; rewrite IHtl. Qed.
 
     Lemma pair_zip_in (T1 T2 : eqType) (s1 : seq T1) (s2 : seq T2) (x0 x : T2) (y1: T1) (i : nat) :
-      size s1 = size s2 -> i < size s2 -> nth x0 s2 i = x -> exists t1, (t1,x) \in zip s1 s2 /\ nth (t1,x0) (zip s1 s2) i = (t1,x).
+      size s1 = size s2 -> i < size s2 -> nth x0 s2 i = x ->
+      exists t1, (t1,x) \in zip s1 s2 /\ nth (t1,x0) (zip s1 s2) i = (t1,x).
     Proof.
     move=> eq_size i_in <-.
     exists (nth y1 s1 i); split.
@@ -243,25 +246,27 @@ relabeling_seq_triple (fun_of_hash_map (color g (init_hash g))) g
 
     Lemma hashes_filter_neq (n m : nat) (hm : hash_map) :
       (m == n) = false ->
-       n \in hashes_hm hm ->
-             n \in hashes_hm (filter (negb \o (fun p0 : B * nat => m == p0.2)) hm).
+        n \in hashes_hm hm ->
+          n \in hashes_hm (filter (negb \o (fun p0 : B * nat => m == p0.2)) hm).
     Proof.
     set p := negb \o (fun p0 : B * nat => m == p0.2).
     elim: hm=> [//| h tl IHtl] /=.
     rewrite in_cons; move=> neq /orP[/eqP eq| in_tl].
     + by rewrite /p/= -eq neq /= in_cons eq eqxx.
-    + case: h=> b n'; rewrite /p/=. case_eq (m != n')=> H; last by apply IHtl.
+    + case: h=> b n'; rewrite /p/=.
+      case_eq (m != n')=> H; last by apply IHtl.
       by rewrite /=; apply inweak; apply IHtl.
     Qed.
 
 
     Lemma partitionate_filter (n m : nat) (hm : hash_map):
       (n == m) = false ->
-      (partitionate n hm).1 = (partitionate n [seq x <- hm | (negb \o eq_hash m) x]).1.
+        (partitionate n hm).1 = (partitionate n [seq x <- hm | (negb \o eq_hash m) x]).1.
     Proof.
     elim: hm=> [//| h tl IHtl] neq; rewrite /=/eq_hash/pred_eq.
     case: ifP=> [/eqP eq_nh2| ]/=; last first.
-    by move=> neq_nh2; rewrite /negb; case: ifP; case: ifP=> //neq_mh2 _ /=; rewrite ?neq_nh2; apply IHtl.
+    + move=> neq_nh2; rewrite /negb.
+      by case: ifP; case: ifP=> //neq_mh2 _ /=; rewrite ?neq_nh2; apply IHtl.
     rewrite eq_sym in neq; rewrite -eq_nh2 neq /= eq_nh2 eqxx; congr cons.
     have -> : [seq p <- tl | h.2 == p.2] = (partitionate h.2 tl).1 by [].
     have -> : [seq p <- [seq x <- tl | m != x.2] | h.2 == p.2] = (partitionate n [seq x <- tl | (negb \o eq_hash m) x]).1.
@@ -291,7 +296,7 @@ relabeling_seq_triple (fun_of_hash_map (color g (init_hash g))) g
         by rewrite orbT.
       have -> : [seq p0 <- tl | n == p0.2] = (partitionate n tl).1 by [].
       rewrite (partitionate_filter n p.2) //; apply IHn.
-      + by apply: leq_ltn_trans measure; apply size_filter.
+      + by apply: leq_ltn_trans measure; apply size_filter_le.
       + by apply hashes_filter_neq=> //; rewrite eq_sym neq_np.
     Qed.
 
@@ -328,7 +333,7 @@ relabeling_seq_triple (fun_of_hash_map (color g (init_hash g))) g
         exact: nat_inj O.
       suffices partP : forall (n : nat) (hm : hash_map), n \in (hashes_hm hm) -> size (partitionate n hm).1 = count (eq_hash n) hm.
         by apply partP; apply mem_nth; apply: ltn_trans lt_ij j_in.
-      by move=> n hm0 nin; rewrite /partitionate/= seq.size_filter.
+      by move=> n hm0 nin; rewrite /partitionate/= size_filter.
     suffices partIn : forall (n : nat) (hm : hash_map), n \in (hashes_hm hm) -> (partitionate n hm).1 \in gen_partition hm.
       by apply partIn ; apply mem_nth; apply: ltn_trans lt_ij j_in.
     by move=> n hm0 nin; apply part_in_partition.
@@ -336,9 +341,9 @@ relabeling_seq_triple (fun_of_hash_map (color g (init_hash g))) g
 
     Lemma nth_funof (g : seq (triple I B L)) (hm : hash_map) :
       bnodes_hm hm =i get_bts g ->
-          is_fine (gen_partition hm) ->
+        is_fine (gen_partition hm) ->
           forall (b : B) dfb dfn (bin : b \in get_bts g),
-      exists n, (nth (dfb, dfn) hm (index b [seq i.1 | i <- hm])) = (b,n).
+            exists n, (nth (dfb, dfn) hm (index b [seq i.1 | i <- hm])) = (b,n).
     Proof.
     move=> mem_eq fine b bdf dfn; rewrite -mem_eq.
     exists (nth dfn [seq i.2 | i <- hm] (index b [seq i.1 | i <- hm])).
@@ -348,8 +353,8 @@ relabeling_seq_triple (fun_of_hash_map (color g (init_hash g))) g
 
     Lemma funof_snd_inj (g : seq (triple I B L)) (hm : hash_map) :
       bnodes_hm hm =i get_bts g ->
-      is_fine (gen_partition hm) ->
-      {in hm &, injective [eta snd]}.
+        is_fine (gen_partition hm) ->
+          {in hm &, injective [eta snd]}.
     Proof.
     rewrite (hm_zip hm).
     set hm' := zip _ _.
@@ -363,49 +368,46 @@ relabeling_seq_triple (fun_of_hash_map (color g (init_hash g))) g
 
     Lemma uniq_get_bts_is_fine (g : seq (triple I B L)) hm :
       bnodes_hm hm =i get_bts g ->
-      is_fine (gen_partition hm) ->
-      uniq [seq fun_of_hash_map hm i | i <- get_bts g].
+        is_fine (gen_partition hm) ->
+          uniq [seq fun_of_hash_map hm i | i <- get_bts g].
     Proof.
     move=> mem_eq fine.
     apply /in_map_injP; first by apply uniq_get_bts.
-    move=> b b' bin b'in.
+    move=> b b'; rewrite -!mem_eq=> bin b'in.
     rewrite /fun_of_hash_map.
-    rewrite -!mem_eq in bin b'in.
-    have  hasb:= (bnodes_hm_has_eq_bnodes _ _ bin).
+    have hasb := (bnodes_hm_has_eq_bnodes _ _ bin).
     have hasb' := (bnodes_hm_has_eq_bnodes _ _ b'in).
-    rewrite hasb hasb'.
-    move=> /nat_inj_.
-    rewrite (hm_zip hm).
+    rewrite hasb hasb' => /nat_inj_.
     have eqsize: size [seq i.2 | i <- hm] = size [seq i.1 | i <- hm] by apply size_proj.
-    rewrite !find_index_eq_bnode //.
-    rewrite -!hm_zip.
-    move=> eq_nth.
+    rewrite (hm_zip hm) !find_index_eq_bnode // -!hm_zip.
+    move=> /eqP.
     have [n nin]:= bnodes_hm_exists hm b bin.
     have [n' n'in]:= bnodes_hm_exists hm b' b'in.
-    move/eqP : eq_nth.
-    suffices [inb inb'] : (index b [seq i.1 | i <- hm] < size hm)%N /\ (index b' [seq i.1 | i <- hm] < size hm)%N.
-    rewrite (nth_map (b,O)) // (nth_map (b',O)) //.
-    have [n'' n''P]: exists n, (nth (b, O) hm (index b [seq i.1 | i <- hm])) = (b,n). by apply (nth_funof g)=> //; rewrite -mem_eq.
-    rewrite n''P.
-    have [n''' n'''P]: exists n, (nth (b', O) hm (index b' [seq i.1 | i <- hm])) = (b',n). by apply (nth_funof g)=> //; rewrite -mem_eq.
-    rewrite n'''P.
-    move=> /eqP eqpair.
-    apply (funof_snd_inj g hm mem_eq fine) in eqpair.
-    by move : eqpair => [->].
-    by rewrite -n''P; apply mem_nth.
-    by rewrite -n'''P; apply mem_nth.
+    suffices [inb inb'] :
+      (index b [seq i.1 | i <- hm] < size hm)%N /\ (index b' [seq i.1 | i <- hm] < size hm)%N.
+      rewrite (nth_map (b,O)) // (nth_map (b',O)) //.
+      have [n'' n''P]: exists n, (nth (b, O) hm (index b [seq i.1 | i <- hm])) = (b,n).
+        by apply (nth_funof g)=> //; rewrite -mem_eq.
+      rewrite n''P.
+      have [n''' n'''P]: exists n, (nth (b', O) hm (index b' [seq i.1 | i <- hm])) = (b',n).
+        by apply (nth_funof g)=> //; rewrite -mem_eq.
+      rewrite n'''P.
+      move=> /eqP /(funof_snd_inj g hm mem_eq fine).
+      rewrite -{1}n''P -{1}n'''P => /(_ (mem_nth _ inb) (mem_nth _ inb')).
+      by move=> [].
     by split; rewrite -(find_index_eq_bnode (map fst hm) (map snd hm)) // -hm_zip -has_find.
     Qed.
 
     Lemma uniq_label_is_fine (g : seq (triple I B L)) (ug: uniq g) (hm : hash_map) :
       bnodes_hm hm =i get_bts g ->
-      is_fine (gen_partition hm) ->
-      uniq (relabeling_seq_triple (fun_of_hash_map hm) g).
-    Proof. move=> mem_eq fine.
-           have := uniq_get_bts_is_fine _ _ mem_eq fine.
-           move=> /(in_map_injP _ (uniq_get_bts _)) mu_inj.
-           rewrite map_inj_in_uniq=> //.
-           by apply inj_get_bts_inj_ts.
+        is_fine (gen_partition hm) ->
+          uniq (relabeling_seq_triple (fun_of_hash_map hm) g).
+    Proof.
+    move=> mem_eq fine.
+    have := uniq_get_bts_is_fine _ _ mem_eq fine.
+    move=> /(in_map_injP _ (uniq_get_bts _)) mu_inj.
+    rewrite map_inj_in_uniq=> //.
+    by apply inj_get_bts_inj_ts.
     Qed.
 
     Equations? distinguish__
@@ -426,10 +428,7 @@ relabeling_seq_triple (fun_of_hash_map (color g (init_hash g))) g
                  if cmp gbot candidate then candidate else gbot in
       foldl_In p f gbot.
       Proof.
-        apply /ltP.
-        rewrite nat_coq_nat.
-        eapply (Order.POrderTheory.le_lt_trans). apply color_refineP.
-        by apply : (markP (s,n)).
+      by apply /ltP; apply (leq_ltn_trans (color_refineP _ _) (markP _ _ inP)).
       Qed.
 
     Definition distinguish (g : seq (triple I B L)) (hm : hash_map) : seq (triple I B L) :=
@@ -450,8 +449,10 @@ relabeling_seq_triple (fun_of_hash_map (color g (init_hash g))) g
 
     Lemma eq_distinguish (g : seq (triple I B L)) (hm : hash_map) :
       distinguish g hm = distinguish_ g hm.
-    Proof. rewrite /distinguish_/distinguish. rewrite -foldl_foldl_eq.
-           autorewrite with distinguish__. by []. Qed.
+    Proof.
+    rewrite /distinguish_/distinguish -foldl_foldl_eq.
+    by autorewrite with distinguish__.
+    Qed.
 
     Definition canonicalize (g : seq (triple I B L)) (hm : hash_map)
       (* (gbot : seq (triple I B L)) *)
@@ -462,7 +463,6 @@ relabeling_seq_triple (fun_of_hash_map (color g (init_hash g))) g
 	        candidate
 	      else (distinguish g hm').
 
-   
     Definition distinguish_fold (g : seq (triple I B L)) (hm : hash_map) : seq (triple I B L) :=
       let p := choose_part hm in
       foldl choose_graph can (map (canonicalize g hm) p).
@@ -473,7 +473,7 @@ relabeling_seq_triple (fun_of_hash_map (color g (init_hash g))) g
 
     Lemma distinguish_fold_map (g : seq (triple I B L)) (hm : hash_map) :
       distinguish g hm = distinguish_fold g hm.
-    Proof. by rewrite /distinguish_fold eq_distinguish /distinguish_  -fold_map /canonicalize. Qed.
+    Proof. by rewrite /distinguish_fold eq_distinguish /distinguish_  -fold_map. Qed.
 
     Definition template (g : seq (triple I B L)) :=
       let hm := init_hash g in
@@ -539,67 +539,65 @@ relabeling_seq_triple (fun_of_hash_map (color g (init_hash g))) g
     Lemma mem_eq_terms_ts (g h : seq (triple I B L)) :
       g =i h -> terms_ts g =i terms_ts h.
     Proof.
-    move=> /= mem_eq t.
-    rewrite /terms_ts.
-    rewrite !mem_undup.
-    apply /idP/idP.
+    move=> mem_eq t.
+    suffices imp ts1 ts2:
+      (forall (t : triple I B L), t \in ts1 -> t \in ts2) ->
+        (forall (trm : term I B L), trm \in terms_ts ts1 -> trm \in terms_ts ts2).
+      by apply /idP/idP; apply imp; move=> ?; rewrite -mem_eq.
+    move=> /= {}mem_eq {}t; rewrite /terms_ts !mem_undup.
     move=> /flatten_mapP /=[t' t'ing tinterm].
-    apply /flatten_mapP=> /=.
-    exists t'. by rewrite -mem_eq. by apply tinterm.
-    move=> /flatten_mapP /=[t' t'ing tinterm].
-    apply /flatten_mapP=> /=.
-    exists t'. by rewrite mem_eq. by apply tinterm.
+    by apply /flatten_mapP=> /=; exists t'=> //; apply mem_eq.
     Qed.
 
     Lemma mem_eq_bnodes_ts (g h : seq (triple I B L)) :
       g =i h -> bnodes_ts g =i bnodes_ts h.
     Proof.
-      move=> /mem_eq_terms_ts mem_eq b; rewrite /bnodes_ts !mem_undup.
-      by rewrite !mem_filter mem_eq.
+    move=> /mem_eq_terms_ts mem_eq b; rewrite /bnodes_ts !mem_undup.
+    by rewrite !mem_filter mem_eq.
     Qed.
 
     Lemma mem_eq_get_bts (g h : seq (triple I B L)) :
       g =i h -> get_bts g =i get_bts h.
     Proof.
-      move=> /mem_eq_bnodes_ts mem_eq b.
-      by apply eq_mem_pmap.
+    move=> /mem_eq_bnodes_ts mem_eq b.
+    by apply eq_mem_pmap.
     Qed.
 
 
     Lemma piso_sort (g: seq (triple I B L)) (mu : B -> B) :
-      is_pre_iso_ts g (sort le_triple (relabeling_seq_triple mu g)) mu <-> is_pre_iso_ts g (relabeling_seq_triple mu g) mu.
+      is_pre_iso_ts g (sort le_triple (relabeling_seq_triple mu g)) mu
+      <-> is_pre_iso_ts g (relabeling_seq_triple mu g) mu.
     Proof.
-      rewrite /is_pre_iso_ts/bnode_map_bij.
-      rewrite !uniq_get_bts/=.
-      split=> H.
-      apply uniq_perm.
-      by rewrite (perm_uniq H) uniq_get_bts.
-      by rewrite uniq_get_bts.
-      move=> b; rewrite (perm_mem H).
-      by apply mem_eq_get_bts=> b'; rewrite mem_sort.
-      apply uniq_perm.
-      by rewrite (perm_uniq H) uniq_get_bts.
-      by rewrite uniq_get_bts.
-      move=> b; rewrite (perm_mem H).
-      by apply mem_eq_get_bts=> b'; rewrite mem_sort.
-      Qed.
+    rewrite /is_pre_iso_ts/bnode_map_bij !uniq_get_bts/=.
+    split=> H.
+    + apply uniq_perm.
+      - by rewrite (perm_uniq H) uniq_get_bts.
+      - by rewrite uniq_get_bts.
+      - move=> b; rewrite (perm_mem H).
+        by apply mem_eq_get_bts=> b'; rewrite mem_sort.
+    + apply uniq_perm.
+      - by rewrite (perm_uniq H) uniq_get_bts.
+      - by rewrite uniq_get_bts.
+      - move=> b; rewrite (perm_mem H).
+        by apply mem_eq_get_bts=> b'; rewrite mem_sort.
+    Qed.
 
     Lemma uniq_map_pre_iso (mu : B -> B) (ts : seq (triple I B L)) :
       uniq (map mu (get_bts ts)) ->
-      is_pre_iso_ts ts (relabeling_seq_triple mu ts) mu.
-    Proof. move=> umu. rewrite /is_pre_iso_ts. rewrite /bnode_map_bij. rewrite !uniq_get_bts /=.
-           apply perm_eq_bts_relabel_inj_in.
-           apply /in_map_injP=> //. apply uniq_get_bts.
-           by apply perm_refl.
+        is_pre_iso_ts ts (relabeling_seq_triple mu ts) mu.
+    Proof.
+    move=> umu; rewrite /is_pre_iso_ts/bnode_map_bij !uniq_get_bts /=.
+    apply perm_eq_bts_relabel_inj_in; last by apply perm_refl.
+    by apply /in_map_injP=> //; apply uniq_get_bts.
     Qed.
 
 
     Lemma piso_funof (g : seq (triple I B L)) (hm: hash_map) :
-        bnodes_hm hm =i get_bts g ->
+      bnodes_hm hm =i get_bts g ->
         is_fine (gen_partition hm) ->
-        is_pre_iso_ts g (relabeling_seq_triple (fun_of_hash_map hm) g) (fun_of_hash_map hm).
+          is_pre_iso_ts g (relabeling_seq_triple (fun_of_hash_map hm) g) (fun_of_hash_map hm).
     Proof.
-      move=> mem_eq fine. apply uniq_map_pre_iso. by apply uniq_get_bts_is_fine.
+    by move=> mem_eq fine; apply uniq_map_pre_iso; apply uniq_get_bts_is_fine.
     Qed.
 
     Lemma init_hash_nil : init_hash [::] = [::].
@@ -627,8 +625,7 @@ relabeling_seq_triple (fun_of_hash_map (color g (init_hash g))) g
     Proof.
     rewrite /template/=; case: ifP; first by [].
     rewrite init_hash_nil. rewrite color_nil_nil.
-    autorewrite with gen_partition.
-    by [].
+    by autorewrite with gen_partition.
     Qed.
 
 
@@ -671,10 +668,12 @@ relabeling_seq_triple (fun_of_hash_map (color g (init_hash g))) g
     by move=> y yin; apply cmp_in; rewrite in_cons yin orbT.
     Qed.
 
-    Hypothesis cmp_can : forall (hm : hash_map) (g y : seq (triple I B L)),
+    Hypothesis cmp_can :
+      forall (hm : hash_map) (g y : seq (triple I B L)),
         y \in [seq canonicalize g hm i | i <- choose_part hm] -> cmp can y.
 
-    Hypothesis choose_from_not_fine : forall (hm : hash_map),
+    Hypothesis choose_from_not_fine :
+      forall (hm : hash_map),
         ~~ is_fine (gen_partition hm) -> choose_part hm == [::] = false.
 
     Lemma nil_is_nil (g : seq (triple I B L)) (hm : hash_map):
@@ -694,139 +693,131 @@ relabeling_seq_triple (fun_of_hash_map (color g (init_hash g))) g
     rewrite distinguish_fold_map.
     move=> /(foldl_can_in_choose _ (cmp_can hm g))/orP[].
     + by rewrite map_nil_is_nil choose_from_not_fine.
-    rewrite /canonicalize.
-    move=> /mapP[/= b bin]; case: ifP.
+    rewrite /canonicalize; move=> /mapP[/= b bin].
+    case: ifP.
     + admit.
     + move=> H /eqP; rewrite eq_sym=> /eqP.
-      apply IHn=> //.
-      apply: Order.POrderTheory.le_lt_trans (color_refineP _ _) _.
+      apply IHn=> //; last by rewrite H.
+      + apply: Order.POrderTheory.le_lt_trans (color_refineP _ _) _.
         by apply: Order.POrderTheory.lt_le_trans (markP _ _ _) measure.
-      by apply color_refine_good_hm; apply good_mark=> //; apply in_part_in_bnodes.
-      by rewrite H.
+      + by apply color_refine_good_hm; apply good_mark=> //; apply in_part_in_bnodes.
     Admitted.
     (* prove this *)
 
     Lemma distinguish_piso (g : seq (triple I B L)) (ug: uniq g):
-        ~~ is_fine (gen_partition (color g (init_hash g))) ->
-      exists mu : B -> B,
-        distinguish g (color g (init_hash g)) = sort le_triple (relabeling_seq_triple mu g) /\
-          is_pre_iso_ts g (distinguish g (color g (init_hash g))) mu.
+      ~~ is_fine (gen_partition (color g (init_hash g))) ->
+        exists mu : B -> B,
+          distinguish g (color g (init_hash g)) = sort le_triple (relabeling_seq_triple mu g)
+          /\ is_pre_iso_ts g (distinguish g (color g (init_hash g))) mu.
     Proof.
-      set hm := (color g (init_hash g)).
-      have : M hm < S (M hm) by apply ltnSn.
-      have : bnodes_hm hm =i get_bts g by apply color_good_hm; apply good_init.
-      move: hm (M hm).+1.
-      move=> hm n; move: n hm=> n.
-      elim: n => [//| n IHn hm' ghm hmM].
-      move: (distinguish_choice g hm')=> /=[].
-      + move=> H finePn. rewrite H. exists id. split. apply (nil_is_nil g _ ghm finePn) in H.
-        by rewrite relabeling_seq_triple_id H.
-        apply (nil_is_nil g _ ghm finePn) in H.
-        rewrite H /is_pre_iso_ts /= /bnode_map_bij.
-        by rewrite (uniq_get_bts _) /= map_id perm_refl.
-      + move=> /mapP/=[bn inp ->].
-        case_eq  (is_fine (gen_partition (color_refine g (mark bn.1 hm'))))=> H.
-        exists (fun_of_hash_map (color_refine g (mark bn.1 hm'))).
-        split=> //.
-        by rewrite /canonicalize H.
-        rewrite /canonicalize H.
-        apply piso_sort.
-        apply piso_funof.
-        apply color_refine_good_hm. apply good_mark=> //.
+    set hm := (color g (init_hash g)).
+    have : M hm < S (M hm) by apply ltnSn.
+    have : bnodes_hm hm =i get_bts g by apply color_good_hm; apply good_init.
+    move: hm (M hm).+1.
+    move=> hm n; move: n hm=> n.
+    elim: n => [//| n IHn hm' ghm hmM] finePn.
+    move: (distinguish_choice g hm')=> /=[].
+    + move=> H; rewrite H; move/(nil_is_nil g _ ghm finePn) : H ->.
+      exists id; split; first by rewrite relabeling_seq_triple_id sort_can.
+      rewrite /is_pre_iso_ts /= /bnode_map_bij.
+      by rewrite (uniq_get_bts _) /= map_id perm_refl.
+    + move=> /mapP/=[bn inp ->].
+      case_eq  (is_fine (gen_partition (color_refine g (mark bn.1 hm'))))=> H.
+      - exists (fun_of_hash_map (color_refine g (mark bn.1 hm'))).
+        rewrite /canonicalize; split=> //; rewrite H //.
+        apply piso_sort; apply piso_funof; last by apply H.
+        apply color_refine_good_hm; apply good_mark=> //.
         by apply in_part_in_bnodes.
-        by apply H.
-      + move=> finePn; rewrite /canonicalize H. apply IHn=> //.
-        apply color_refine_good_hm.
-        apply good_mark=> //.
+      - rewrite /canonicalize H; apply IHn=> //; last by rewrite H.
+        apply color_refine_good_hm; apply good_mark=> //.
         by apply in_part_in_bnodes.
-        eapply Order.POrderTheory.le_lt_trans.
-        apply color_refineP.
-        eapply Order.POrderTheory.lt_le_trans.
-        by apply markP.
-        by apply hmM.
-        by rewrite H.
+      eapply Order.POrderTheory.le_lt_trans; first by apply color_refineP.
+      by apply (Order.POrderTheory.lt_le_trans (markP _ _ inp) hmM).
     Qed.
 
     Lemma preiso_out_template (g : seq (triple I B L)) (ug : uniq g) :
-      exists mu, (template g) = sort le_triple (relabeling_seq_triple mu g) /\ is_pre_iso_ts g (template g) mu.
+      exists mu, (template g) = sort le_triple (relabeling_seq_triple mu g)
+                 /\ is_pre_iso_ts g (template g) mu.
     Proof.
-      move/eqP : (eq_refl (template g)).
-      rewrite {2}/template.
-      case: ifP=> is_fine ->.
-      exists (fun_of_hash_map (color g (init_hash g))).
-      split=> //. apply piso_sort. apply piso_funof=> //.
-      apply color_good_hm; apply good_init.
-      by apply distinguish_piso=> //; rewrite is_fine.
+    move/eqP : (eq_refl (template g)).
+    rewrite {2}/template.
+    case: ifP=> is_fine ->.
+    exists (fun_of_hash_map (color g (init_hash g))); split=> //.
+    + apply piso_sort; apply piso_funof=> //.
+      by apply color_good_hm; apply good_init.
+    by apply distinguish_piso=> //; rewrite is_fine.
     Qed.
 
     Lemma eiso_sort (g: seq (triple I B L)) (mu : B -> B) :
-        is_effective_iso_ts g (relabeling_seq_triple mu g) mu ->
-        is_effective_iso_ts g (sort le_triple (relabeling_seq_triple mu g)) mu.
-    Proof. move=> /and3P/= [piso urel peq].
-           apply /and3P; split=> //.
-           by apply piso_sort.
-           apply uniq_perm=> //.
-           by rewrite sort_uniq.
-           by move=> b; rewrite mem_sort.
+      is_effective_iso_ts g (relabeling_seq_triple mu g) mu ->
+      is_effective_iso_ts g (sort le_triple (relabeling_seq_triple mu g)) mu.
+    Proof.
+    move=> /and3P/= [piso urel peq].
+    apply /and3P; split=> //; first by apply piso_sort.
+    apply uniq_perm=> //; first by rewrite sort_uniq.
+    by move=> b; rewrite mem_sort.
     Qed.
 
-    Lemma eiso_out_template (g : seq (triple I B L)) (ug : uniq g) : effective_iso_ts g (template g).
+    Lemma eiso_out_template (g : seq (triple I B L)) (ug : uniq g) :
+      effective_iso_ts g (template g).
     Proof.
-      rewrite /iso_ts.
-      move: (uniq_template g ug).
-      suffices [mu  [-> piso utg]]: exists mu, (template g) = sort le_triple (relabeling_seq_triple mu g) /\ is_pre_iso_ts g (template g) mu.
+    rewrite /iso_ts.
+    move: (uniq_template g ug).
+    suffices [mu  [-> piso utg]]:
+      exists mu, (template g) = sort le_triple (relabeling_seq_triple mu g)
+                 /\ is_pre_iso_ts g (template g) mu.
       rewrite sort_uniq in utg.
       exists mu; apply eiso_sort.
-      have {}piso : is_pre_iso_ts g (relabeling_seq_triple mu g) mu. apply piso_sort in piso. by apply piso.
-      move : (ts_pre_iso_effective_iso utg piso)=> eiso //.
-      by apply preiso_out_template.
+      have {}piso : is_pre_iso_ts g (relabeling_seq_triple mu g) mu by apply piso_sort.
+      by move : (ts_pre_iso_effective_iso utg piso)=> eiso //.
+    by apply preiso_out_template.
     Qed.
 
-
-    Hypothesis iso_color_fine : forall (g h : seq (triple I B L)),
-      uniq g -> uniq h ->
-      effective_iso_ts g h ->
-      is_fine (gen_partition (color g (init_hash g))) =
-        is_fine (gen_partition (color h (init_hash h))).
-
-    Hypothesis distinguish_complete : forall (g h : seq (triple I B L)),
+    Hypothesis iso_color_fine :
+      forall (g h : seq (triple I B L)),
         uniq g -> uniq h ->
-        effective_iso_ts g h ->
-        is_fine (gen_partition (color g (init_hash g))) = false ->
-        distinguish g (color g (init_hash g)) == distinguish h (color h (init_hash h)).
+          effective_iso_ts g h ->
+            is_fine (gen_partition (color g (init_hash g)))
+            = is_fine (gen_partition (color h (init_hash h))).
+
+    Hypothesis distinguish_complete :
+      forall (g h : seq (triple I B L)),
+        uniq g -> uniq h ->
+          effective_iso_ts g h ->
+            is_fine (gen_partition (color g (init_hash g))) = false ->
+              distinguish g (color g (init_hash g)) == distinguish h (color h (init_hash h)).
 
 
-    Hypothesis eiso_mem_eq_canonicalize : forall (g h : seq (triple I B L)) (ug: uniq g) (uh: uniq h),
+    Hypothesis eiso_mem_eq_canonicalize :
+      forall (g h : seq (triple I B L)) (ug: uniq g) (uh: uniq h),
         effective_iso_ts g h ->
-        is_fine (gen_partition (color g (init_hash g))) = false ->
-        map (canonicalize g (color g (init_hash g))) (choose_part (color g (init_hash g))) =i
-             map (canonicalize h (color h (init_hash h))) (choose_part (color h (init_hash h))).
+          is_fine (gen_partition (color g (init_hash g))) = false ->
+            map (canonicalize g (color g (init_hash g))) (choose_part (color g (init_hash g)))
+            =i map (canonicalize h (color h (init_hash h))) (choose_part (color h (init_hash h))).
 
     Lemma eiso_correct_complete (g h : seq (triple I B L)) (ug: uniq g) (uh: uniq h) :
       effective_iso_ts g h <-> (template g) == (template h).
     Proof.
-      split; last first.
-      move=> /eqP eqmgmh.
+    split; last first.
+    + move=> /eqP eqmgmh.
       have := eiso_out_template g ug.
       rewrite eqmgmh=> mgh.
       have /(effective_iso_ts_sym uh) hmh := eiso_out_template h uh.
       by apply: (effective_iso_ts_trans mgh hmh).
-      rewrite /template=> eiso.
-      rewrite -(iso_color_fine _ _ eiso) //.
-      case: ifP.
-      move=> is_fineP.
-      apply /eqP/rdf_leP.
+    rewrite /template=> eiso.
+    rewrite -(iso_color_fine _ _ eiso) //.
+    case: ifP=> [fineP|finePn].
+    + apply /eqP/rdf_leP.
       apply uniq_perm.
-      apply uniq_label_is_fine=> //. apply color_good_hm. apply good_init.
-      rewrite (iso_color_fine _ _ eiso) // in is_fineP.
-      apply uniq_label_is_fine=> //. apply color_good_hm. apply good_init.
-      by apply iso_color_fine_can.
-      move=> is_finePn.
-      rewrite !distinguish_fold_map /distinguish_fold.
+      - by apply uniq_label_is_fine=> //; apply color_good_hm; apply good_init.
+      - rewrite (iso_color_fine _ _ eiso) // in fineP.
+        by apply uniq_label_is_fine=> //; apply color_good_hm; apply good_init.
+        by apply iso_color_fine_can.
+    + rewrite !distinguish_fold_map /distinguish_fold.
       set cang := (map _ (choose_part (color g (init_hash g)))).
       set canh := (map _ (choose_part (color h (init_hash h)))).
       suffices mem_eq : cang =i canh.
-      by rewrite !foldl_idx (eq_big_idem (fun x => true) _ choose_graph_idem mem_eq) eqxx.
+        by rewrite !foldl_idx (eq_big_idem _ _ choose_graph_idem mem_eq) eqxx.
       by apply eiso_mem_eq_canonicalize.
     Qed.
 
